Logic/MultiSuccCorsiTassi/Correctness.lean
@@ -14,7 +14,7 @@ open multiSucc
 
 /- TODO: problem with showing impr correctness, because of blocked implication semantics -/
 theorem proof_correctness :
-  ∀ (s : Sequent) (_ : Proof s) (m : Model) (_ : m.wf), s.eval m ≠ TV.f := by
+  ∀ (s : Sequent) (_ : Proof s) (m : Model) (_ : m.wf), s.evalP m ≠ TV.f := by
   intro s pf m wf
   induction pf generalizing m with
   | ax x xs ys bl hxs hys =>
@@ -24,62 +24,80 @@ theorem proof_correctness :
       suffices evalSucc ↑ys m = TV.t by grind
       apply evalSucc_true hys
       grind
-    else if xtv' : x ∈ m.world.unforced then grind
+    else if xtv' : x ∈ m.world.rejected then grind
     else grind
-  | botl => grind
-  | botr xs ys prem => simp_all
-  | andl a b xs ys prem ih =>
-    simp_all
-  | andr a b xs ys prem1 prem2 =>
-    simp_all only [ne_eq, Sequent.eval_false_iff]
+  | botl xs ys bl =>
+    have hAnt : evalAnt ({ Γa := ↑(⊥ :: xs), Γb := ↑bl, Δ := ↑ys } : Sequent).Γ m = TV.f := by
+      apply evalAnt_false (f := ⊥)
+      · simp [Sequent.Γ]
+      · simp
     grind
-  | orl a b xs ys prem1 prem2 =>
-    simp_all only [ne_eq, Sequent.eval_false_iff, not_and]
+  | botr xs ys prem => simp_all
+  | andl a b xs ys bl prem ih =>
+    simp_all
+    specialize ih m wf
+    intro h
+    apply ih
+    intro x hx
+    rcases hx with (⟨rfl, _⟩ | ⟨rfl, _⟩ | hx) | hbl
+    · have hab : (a ∧∧ b).eval m = TV.t := h (a ∧∧ b) (by simp)
+      rw [evaluate_and, conjTV_true_iff] at hab
+      exact hab.1
+    · have hab : (a ∧∧ b).eval m = TV.t := h (a ∧∧ b) (by simp)
+      rw [evaluate_and, conjTV_true_iff] at hab
+      exact hab.2
+    · exact h x (by simp [hx])
+    · exact h x (by simp [hbl])
+  | andr a b xs ys prem1 prem2 =>
+    simp_all only [ne_eq, Sequent.evalP_false_iff]
+    grind
+  | orl a b xs ys bl prem1 prem2 ih₁ ih₂ =>
+    simp_all only [ne_eq, Sequent.evalP_false_iff, not_and]
+    simp_all
+    specialize ih₁ m wf
+    specialize ih₂ m wf
+    intro h
+    have hor : (a ∨∨ b).eval m = TV.t := h (a ∨∨ b) (by simp)
+    rw [evaluate_or, disjTV_true_iff] at hor
     grind
   | orr a b xs ys prem =>
     simp_all
   | impr a b xs ys bl prem ih =>
     apply eval_imp_righ_wo_ys
     simp_all
-    intro h₁ h₂ impF
+    intro h₁ impF
     apply eval_imp_false_contradict at impF
-    rcases impF with ⟨m', m'_in, h₃, h₄⟩
-    specialize ih m' (by grind) h₃
+    contrapose! ih
     simp_all
-    rcases ih with ⟨x, (_ | ⟨x, xbl, _, _⟩), xeval⟩
-    . grind [Model.mono_all_true]
-    . clear h₁ h₃ h₄
-      contrapose xeval
-      specialize h₂ x xbl
-      sorry
-      --exact evalBlocked_true_in_branch (i := x) (m := m) (m' := m') wf m'_in h₂
+    rcases impF with ⟨m', m'_in, h₃, h₄⟩
+    . use m'
+      simp_all
+      constructor
+      . grind only [Model.all_wf]
+      . intro x h; specialize h₁ x  h
+        grind [Model.mono_all_true]
 
   | impl a b xs ys bl prem1 prem2 ih₁ ih₂ =>
     simp_all
-    intro h₁ h₂
-    have impT := h₁
-    rw [eval_imp_true_iff] at h₁
-    simp at h₁
-    cases h₁ with
-    | intro himp hbranch =>
-      cases himp with
-      | inl h =>
-        intro hbl
-        apply ih₁ <;> try grind [evalBlocked_true_iff]
-      | inr h => simp_all
+    intro h₁
+    specialize ih₁ m wf
+    specialize ih₂ m wf
+    have hImp : (a ⊃ b).eval m = TV.t := h₁ (a ⊃ b) (by simp)
+    grind
 
   | afort a b xs ys bl prem ih =>
-    simp_all
-    intro h₁ h₂ i
-    specialize ih m wf h₁ h₂
+    simp
+    simp at ih
+    intro h₁ h₂
+    specialize ih m wf h₁
     apply_assumption
-    apply imp_false_then_b_false i wf
+    apply imp_false_then_b_false h₂ wf
 
 #print axioms proof_correctness
 
 /- test proof for only the truth value. Here ax case can currently not be proved -/
 theorem proof_correctness' :
-  ∀ (s : Sequent) (_ : Proof s) (m : Model) (_ : m.wf), s.eval m = TV.t := by
+  ∀ (s : Sequent) (_ : Proof s) (m : Model) (_ : m.wf), s.evalP m = TV.t := by
   intro s pf m wf
   induction pf generalizing m with
   | ax x xs ys bl hxs hys =>
@@ -89,9 +107,14 @@ theorem proof_correctness' :
       suffices evalSucc ↑ys m = TV.t by grind
       apply evalSucc_true hys
       grind
-    else if xtv' : x ∈ m.world.unforced then grind
+    else if xtv' : x ∈ m.world.rejected then grind
     else sorry
-  | botl => grind
+  | botl xs ys bl =>
+    have hAnt : evalAnt ({ Γa := ↑(⊥ :: xs), Γb := ↑bl, Δ := ↑ys } : Sequent).Γ m = TV.f := by
+      apply evalAnt_false (f := ⊥)
+      · simp [Sequent.Γ]
+      · simp
+    grind
   | botr xs ys prem => simp_all
   | andl a b xs ys bl prem ih =>
     simp_all; specialize ih m wf; grind
@@ -117,50 +140,30 @@ theorem proof_correctness' :
         sorry
     . left
       rcases h₂ with x_xs | ⟨x_bl, h, _, _⟩
-      . left; grind
-      . right
-        rw [eval_imp_false_iff] at xtv
-        use x_bl; simp_all
-        rw [evalBlocked_false_iff]
-        sorry
+      . use x; grind
+      . let x := x_bl.f ⊃ x_bl.g
+        use x; grind
     . right
-      sorry
+      grind [b_true_then_imp_true_branch]
 
   | impl a b xs ys bl prem1 prem2 ih₁ ih₂ =>
     simp_all
     specialize ih₁ m wf
     specialize ih₂ m wf
-    rcases ih₂ with h₂ | hys
-    · rcases h₂ with hbf | hbl
-      · rcases hbf with hb | hxs
-        · rcases ih₁ with h₁ | hys
-          · rcases h₁ with hxs | himp | hbl
-            · exact Or.inl <| Or.inl <| Or.inr hxs
-            · have hImpF : (a ⊃ b).eval m = TV.f := by
-                rw [eval_imp_false_iff]
-                right
-                exact (evalBlocked_false_iff (x := ⟨a, b⟩) (m := m)).1 himp
-              exact Or.inl <| Or.inl <| Or.inl hImpF
-            · exact Or.inl <| Or.inr hbl
-          · rcases hys with hat | hys
-            · have hImpF : (a ⊃ b).eval m = TV.f := by
-                rw [eval_imp_false_iff]
-                left
-                exact ⟨hat, hb⟩
-              exact Or.inl <| Or.inl <| Or.inl hImpF
-            · exact Or.inr hys
-        · exact Or.inl <| Or.inl <| Or.inr hxs
-      · exact Or.inl <| Or.inr hbl
-    · exact Or.inr hys
+    rcases ih₁ with ⟨x, hx, hxf⟩ | ha | hys
+    · left; use x; grind
+    . rcases ih₂ with ⟨x, hx, hxf⟩ | hys
+      · left
+        sorry
+      . right; exact hys
+    · right; exact hys
 
   | afort a b xs ys bl prem ih =>
     simp_all
     specialize ih m wf
-    rcases ih with (ih₁ | ih₁) | ih₁ | ih₁
-    . left; left; apply_assumption
-    . left; right; apply_assumption
-    . right; left
-      apply b_true_then_imp_true_branch wf ih₁
-    . right; right; apply_assumption
+    rcases ih with ⟨x, hx, hxf⟩ | hb | hys
+    . left; grind
+    . right;  left; grind [b_true_then_imp_true_branch]
+    . right; right; exact hys
 
 end multiSucc
